@prefix cc: <http://creativecommons.org/ns#> .
@prefix csvw: <http://www.w3.org/ns/csvw#> .
@prefix ctag: <http://commontag.org/ns#> .
@prefix dc: <http://purl.org/dc/terms/> .
@prefix dc11: <http://purl.org/dc/elements/1.1/> .
@prefix dcat: <http://www.w3.org/ns/dcat#> .
@prefix dcterms: <http://purl.org/dc/terms/> .
@prefix foaf: <http://xmlns.com/foaf/0.1/> .
@prefix gr: <http://purl.org/goodrelations/v1#> .
@prefix grddl: <http://www.w3.org/2003/g/data-view#> .
@prefix ical: <http://www.w3.org/2002/12/cal/icaltzd#> .
@prefix ma: <http://www.w3.org/ns/ma-ont#> .
@prefix og: <http://ogp.me/ns#> .
@prefix org: <http://www.w3.org/ns/org#> .
@prefix owl: <http://www.w3.org/2002/07/owl#> .
@prefix prov: <http://www.w3.org/ns/prov#> .
@prefix qb: <http://purl.org/linked-data/cube#> .
@prefix rdf: <http://www.w3.org/1999/02/22-rdf-syntax-ns#> .
@prefix rdfa: <http://www.w3.org/ns/rdfa#> .
@prefix rdfs: <http://www.w3.org/2000/01/rdf-schema#> .
@prefix rev: <http://purl.org/stuff/rev#> .
@prefix rif: <http://www.w3.org/2007/rif#> .
@prefix rr: <http://www.w3.org/ns/r2rml#> .
@prefix schema: <http://schema.org/> .
@prefix sd: <http://www.w3.org/ns/sparql-service-description#> .
@prefix sioc: <http://rdfs.org/sioc/ns#> .
@prefix skos: <http://www.w3.org/2004/02/skos/core#> .
@prefix skosxl: <http://www.w3.org/2008/05/skos-xl#> .
@prefix v: <http://rdf.data-vocabulary.org/#> .
@prefix vcard: <http://www.w3.org/2006/vcard/ns#> .
@prefix void: <http://rdfs.org/ns/void#> .
@prefix wdr: <http://www.w3.org/2007/05/powder#> .
@prefix wrds: <http://www.w3.org/2007/05/powder-s#> .
@prefix xhv: <http://www.w3.org/1999/xhtml/vocab#> .
@prefix xml: <http://www.w3.org/XML/1998/namespace> .
@prefix xsd: <http://www.w3.org/2001/XMLSchema#> .

# CSVM Ontology definition
csvw: a owl:Ontology;
  dc:title "Metadata Vocabulary for Tabular Data"@en;
  dc:description """Validation, conversion, display and search of tabular data on the web
    requires additional metadata that describes how the data should be
    interpreted. This document defines a vocabulary for metadata that
    annotates tabular data. This can be used to provide metadata at various
    levels, from collections of data from CSV documents and how they relate
    to each other down to individual cells within a table."""@en;
  .


# Class definitions
csvw:Column a rdfs:Class;
  rdfs:label "Column Description"@en;
  rdfs:comment """A Column Description describes a single column."""@en;
  rdfs:isDefinedBy csvw: .
csvw:Dialect a rdfs:Class;
  rdfs:label "Dialect Description"@en;
  rdfs:comment """A Dialect Description provides hints to parsers about how to parse a linked file."""@en;
  rdfs:isDefinedBy csvw: .
csvw:Direction a rdfs:Class;
  rdfs:label "Direction"@en;
  rdfs:comment """The class of table/text directions."""@en;
  rdfs:isDefinedBy csvw: .
csvw:Schema a rdfs:Class;
  rdfs:label "Schema"@en;
  rdfs:comment """A Schema is a definition of a tabular format that may be common to multiple tables."""@en;
  rdfs:isDefinedBy csvw: .
csvw:Table a rdfs:Class;
  rdfs:label "Table Description"@en;
  rdfs:comment """A table description is a JSON object that describes a table within a CSV file."""@en;
  rdfs:isDefinedBy csvw: .
csvw:TableGroup a rdfs:Class;
  rdfs:label "Table Group Description"@en;
  rdfs:comment """A Table Group Description describes a group of Tables."""@en;
  rdfs:isDefinedBy csvw: .
csvw:Template a rdfs:Class;
  rdfs:label "Template Specification"@en;
  rdfs:comment """A Template Specification is a definition of how tabular data can be transformed into another format."""@en;
  rdfs:isDefinedBy csvw: .

# Property definitions
csvw:aboutUrl a rdf:Property;
  rdfs:label "about URL"@en;
  rdfs:comment """A URI template property that may be used to create a unique identifier for each cell within a row when mapping data to other formats"""@en;
  rdfs:domain [ owl:unionOf (csvw:TableGroup csvw:Table csvw:Schema csvw:Column)];
  rdfs:range csvw:uriTemplate;
  rdfs:isDefinedBy csvw: .
csvw:columns a rdf:Property;
  rdfs:label "columns"@en;
  rdfs:comment """An array of Column Descriptions."""@en;
  rdfs:domain csvw:Schema;
  rdfs:range csvw:Column;
  rdfs:isDefinedBy csvw: .
csvw:commentPrefix a rdf:Property;
  rdfs:label "comment prefix"@en;
  rdfs:comment """A character that, when it appears at the beginning of a skipped row, indicates a comment that should be associated as a comment annotation to the table. The default is "#"."""@en;
  rdfs:domain csvw:Dialect;
  rdfs:range xsd:string;
  rdfs:isDefinedBy csvw: .
csvw:datatype a rdf:Property;
  rdfs:label "datatype"@en;
  rdfs:comment """The main datatype of the values of the cell. If the cell contains a list (ie separator is specified and not null) then this is the datatype of each value within the list."""@en;
  rdfs:domain [ owl:unionOf (csvw:TableGroup csvw:Table csvw:Schema csvw:Column)];
  rdfs:range rdfs:Datatype;
  rdfs:isDefinedBy csvw: .
csvw:default a rdf:Property;
  rdfs:label "default"@en;
  rdfs:comment """An atomic property holding a single string that provides a default string value for the cell in cases where the original string value is a null value. This default value may be used when converting the table into other formats."""@en;
  rdfs:domain [ owl:unionOf (csvw:TableGroup csvw:Table csvw:Schema csvw:Column)];
  rdfs:range xsd:string;
  rdfs:isDefinedBy csvw: .
csvw:delimiter a rdf:Property;
  rdfs:label "delimiter"@en;
  rdfs:comment """The separator between cells. The default is ","."""@en;
  rdfs:domain csvw:Dialect;
  rdfs:range xsd:string;
  rdfs:isDefinedBy csvw: .
csvw:dialect a rdf:Property;
  rdfs:label "dialect"@en;
  rdfs:comment """Provides hints to processors about how to parse the referenced files for to create tabular data models for an individual table, or all the tables in a group."""@en;
  rdfs:domain [ owl:unionOf (csvw:TableGroup csvw:Table)];
  rdfs:range csvw:Dialect;
  rdfs:isDefinedBy csvw: .
csvw:doubleQuote a rdf:Property;
  rdfs:label "double quote"@en;
  rdfs:comment """If true, sets the escape character flag to ". If false, to \\."""@en;
  rdfs:domain csvw:Dialect;
  rdfs:range xsd:boolean;
  rdfs:isDefinedBy csvw: .
csvw:encoding a rdf:Property;
  rdfs:label "encoding"@en;
  rdfs:comment """The character encoding for the file, one of the encodings listed in [encoding]. The default is utf-8."""@en;
  rdfs:domain csvw:Dialect;
  rdfs:range xsd:string;
  rdfs:isDefinedBy csvw: .
csvw:foreignKeys a rdf:Property;
  rdfs:label "foreign keys"@en;
  rdfs:comment """An array of foreign key definitions that define how the values from specified columns within this table link to rows within this table or other tables."""@en;
  rdfs:domain csvw:Schema;
  rdfs:range xsd:string;
  rdfs:isDefinedBy csvw: .
csvw:format a rdf:Property;
  rdfs:label "format"@en;
  rdfs:comment """A definition of the format of the cell, used when parsing the cell."""@en;
  rdfs:domain [ owl:unionOf (csvw:TableGroup csvw:Table csvw:Schema csvw:Column)];
  rdfs:range xsd:string;
  rdfs:isDefinedBy csvw: .
csvw:header a rdf:Property;
  rdfs:label "header"@en;
  rdfs:comment """"""@en;
  rdfs:domain csvw:Dialect;
  rdfs:range xsd:boolean;
  rdfs:isDefinedBy csvw: .
csvw:headerColumnCount a rdf:Property;
  rdfs:label "header column count"@en;
  rdfs:comment """The number of header columns (following the skipped columns) in each row. The default is 0.
"""@en;
  rdfs:domain csvw:Dialect;
  rdfs:range xsd:nonNegativeInteger;
  rdfs:isDefinedBy csvw: .
csvw:headerRowCount a rdf:Property;
  rdfs:label "header row count"@en;
  rdfs:comment """The number of header rows (following the skipped rows) in the file. The default is 1."""@en;
  rdfs:domain csvw:Dialect;
  rdfs:range xsd:nonNegativeInteger;
  rdfs:isDefinedBy csvw: .
csvw:language a rdf:Property;
  rdfs:label "language"@en;
  rdfs:comment """A language code as defined by [BCP47]. Indicates the language of the value within the cell."""@en;
  rdfs:domain [ owl:unionOf (csvw:TableGroup csvw:Table csvw:Schema csvw:Column)];
  rdfs:range xsd:string;
  rdfs:isDefinedBy csvw: .
csvw:length a rdf:Property;
  rdfs:label "length"@en;
  rdfs:comment """The exact length of the value of the cell."""@en;
  rdfs:domain [ owl:unionOf (csvw:TableGroup csvw:Table csvw:Schema csvw:Column)];
  rdfs:range xsd:nonNegativeInteger;
  rdfs:isDefinedBy csvw: .
csvw:lineTerminator a rdf:Property;
  rdfs:label "line terminator"@en;
  rdfs:comment """The character that is used at the end of a row. The default is CRLF."""@en;
  rdfs:domain csvw:Dialect;
  rdfs:range xsd:string;
  rdfs:isDefinedBy csvw: .
csvw:maxExclusive a rdf:Property;
  rdfs:label "max exclusive"@en;
  rdfs:comment """The maximum value for the cell (exclusive)."""@en;
  rdfs:domain [ owl:unionOf (csvw:TableGroup csvw:Table csvw:Schema csvw:Column)];
  rdfs:range xsd:integer;
  rdfs:isDefinedBy csvw: .
csvw:maxInclusive a rdf:Property;
  rdfs:label "max inclusive"@en;
  rdfs:comment """The maximum value for the cell (inclusive). """@en;
  rdfs:domain [ owl:unionOf (csvw:TableGroup csvw:Table csvw:Schema csvw:Column)];
  rdfs:range xsd:integer;
  rdfs:isDefinedBy csvw: .
csvw:maxLength a rdf:Property;
  rdfs:label "max length"@en;
  rdfs:comment """The maximum length of the value of the cell."""@en;
  rdfs:domain [ owl:unionOf (csvw:TableGroup csvw:Table csvw:Schema csvw:Column)];
  rdfs:range xsd:nonNegativeInteger;
  rdfs:isDefinedBy csvw: .
csvw:minExclusive a rdf:Property;
  rdfs:label "min exclusive"@en;
  rdfs:comment """The minimum value for the cell (exclusive)."""@en;
  rdfs:domain [ owl:unionOf (csvw:TableGroup csvw:Table csvw:Schema csvw:Column)];
  rdfs:range xsd:integer;
  rdfs:isDefinedBy csvw: .
csvw:minInclusive a rdf:Property;
  rdfs:label "min inclusive"@en;
  rdfs:comment """The minimum value for the cell (inclusive)."""@en;
  rdfs:domain [ owl:unionOf (csvw:TableGroup csvw:Table csvw:Schema csvw:Column)];
  rdfs:range xsd:integer;
  rdfs:isDefinedBy csvw: .
csvw:minLength a rdf:Property;
  rdfs:label "min length"@en;
  rdfs:comment """The minimum length of the value of the cell."""@en;
  rdfs:domain [ owl:unionOf (csvw:TableGroup csvw:Table csvw:Schema csvw:Column)];
  rdfs:range xsd:nonNegativeInteger;
  rdfs:isDefinedBy csvw: .
csvw:name a rdf:Property;
  rdfs:label "name"@en;
  rdfs:comment """An atomic property that gives a canonical name for the column. This must be a string. Conversion specifications must use this property as the basis for the names of properties/elements/attributes in the results of conversions."""@en;
  rdfs:domain csvw:Column;
  rdfs:range xsd:string;
  rdfs:isDefinedBy csvw: .
csvw:notes a rdf:Property;
  rdfs:label "notes"@en;
  rdfs:comment """An array of objects representing annotations. This specification does not place any constraints on the structure of these objects."""@en;
  rdfs:domain csvw:Table;
  rdfs:isDefinedBy csvw: .
csvw:null a rdf:Property;
  rdfs:label "null"@en;
  rdfs:comment """The string used for null values. If not specified, the default for this is the empty string."""@en;
  rdfs:domain [ owl:unionOf (csvw:TableGroup csvw:Table csvw:Schema csvw:Column)];
  rdfs:range xsd:string;
  rdfs:isDefinedBy csvw: .
csvw:propertyUrl a rdf:Property;
  rdfs:label "property URL"@en;
  rdfs:comment """An URI template property that holds one or more strings that may be expanded to URIs for properties if the table is mapped to another format. The default value of propertyUrl is "{#_name}"."""@en;
  rdfs:domain [ owl:unionOf (csvw:TableGroup csvw:Table csvw:Schema csvw:Column)];
  rdfs:range csvw:uriTemplate;
  rdfs:isDefinedBy csvw: .
csvw:primaryKey a rdf:Property;
  rdfs:label "primary key"@en;
  rdfs:comment """A column reference property that holds either a single reference to a column description object or an array of references."""@en;
  rdfs:domain csvw:Schema;
  rdfs:range xsd:string;
  rdfs:isDefinedBy csvw: .
csvw:quoteChar a rdf:Property;
  rdfs:label "quote char"@en;
  rdfs:comment """The character that is used around escaped cells."""@en;
  rdfs:domain csvw:Dialect;
  rdfs:range xsd:string;
  rdfs:isDefinedBy csvw: .
csvw:required a rdf:Property;
  rdfs:label "required"@en;
  rdfs:comment """A boolean value which indicates whether every cell within the column must have a non-null value."""@en;
  rdfs:domain csvw:Column;
  rdfs:range xsd:boolean;
  rdfs:isDefinedBy csvw: .
csvw:resources a rdf:Property;
  rdfs:label "resources"@en;
  rdfs:comment """An array of table descriptions for the tables in the group."""@en;
  rdfs:domain csvw:TableGroup;
  rdfs:range csvw:Table;
  rdfs:isDefinedBy csvw: .
csvw:row a rdf:Property;
  rdfs:label "row"@en;
  rdfs:comment """Relates a Table to each Row output."""@en;
  rdfs:subPropertyOf rdfs:member;
  rdfs:domain csvw:Table;
  rdfs:isDefinedBy csvw: .
csvw:tableSchema a rdf:Property;
  rdfs:label "table schema"@en;
  rdfs:comment """An object property that provides a schema description for an individual table, or all the tables in a group."""@en;
  rdfs:domain [ owl:unionOf (csvw:TableGroup csvw:Table)];
  rdfs:range csvw:Schema;
  rdfs:isDefinedBy csvw: .
csvw:separator a rdf:Property;
  rdfs:label "separator"@en;
  rdfs:comment """The character used to separate items in the string value of the cell."""@en;
  rdfs:domain [ owl:unionOf (csvw:TableGroup csvw:Table csvw:Schema csvw:Column)];
  rdfs:range xsd:string;
  rdfs:isDefinedBy csvw: .
csvw:skipBlankRows a rdf:Property;
  rdfs:label "skip blank rows"@en;
  rdfs:comment """Indicates whether to ignore wholly empty rows (ie rows in which all the cells are empty). The default is false."""@en;
  rdfs:domain csvw:Dialect;
  rdfs:range xsd:boolean;
  rdfs:isDefinedBy csvw: .
csvw:skipColumns a rdf:Property;
  rdfs:label "skip columns"@en;
  rdfs:comment """The number of columns to skip at the beginning of each row, before any header columns. The default is 0."""@en;
  rdfs:domain csvw:Dialect;
  rdfs:range xsd:nonNegativeInteger;
  rdfs:isDefinedBy csvw: .
csvw:skipInitialSpace a rdf:Property;
  rdfs:label "skip initial space"@en;
  rdfs:comment """If true, sets the trim flag to "start". If false, to false."""@en;
  rdfs:domain csvw:Dialect;
  rdfs:range xsd:boolean;
  rdfs:isDefinedBy csvw: .
csvw:skipRows a rdf:Property;
  rdfs:label "skip rows"@en;
  rdfs:comment """The number of rows to skip at the beginning of the file, before a header row or tabular data."""@en;
  rdfs:domain csvw:Dialect;
  rdfs:range xsd:nonNegativeInteger;
  rdfs:isDefinedBy csvw: .
csvw:source a rdf:Property;
  rdfs:label "source"@en;
  rdfs:comment """The format to which the tabular data should be transformed prior to the transformation using the template. If the value is "json", the tabular data should first be transformed first to JSON based on the simple mapping defined in Generating JSON from Tabular Data on the Web. If the value is "rdf", it should similarly first be transformed to XML based on the simple mapping defined in Generating RDF from Tabular Data on the Web."""@en;
  rdfs:domain csvw:Template;
  rdfs:range xsd:string;
  rdfs:isDefinedBy csvw: .
csvw:table a rdf:Property;
  rdfs:label "table"@en;
  rdfs:comment """Relates an Table group to annotated tables. (Note, this is different from csvw:resources, which relates metadata, rather than resulting annotated table descriptions."""@en;
  rdfs:subPropertyOf rdfs:member;
  rdfs:domain csvw:TableGroup;
  rdfs:range csvw:Table;
  rdfs:isDefinedBy csvw: .
csvw:table-direction a rdf:Property;
  rdfs:label "table direction"@en;
  rdfs:comment """One of csvw:rtl csvw:ltr or csvw:default. Indicates whether the tables in the group should be displayed with the first column on the right, on the left, or based on the first character in the table that has a specific direction. """@en;
  rdfs:domain [ owl:unionOf (csvw:TableGroup csvw:Table)];
  rdfs:range csvw:Direction;
  rdfs:isDefinedBy csvw: .
csvw:targetFormat a rdf:Property;
  rdfs:label "target format"@en;
  rdfs:comment """A URL for the format that will be created through the transformation. If one has been defined, this should be a URL for a media type, in the form http://www.iana.org/assignments/media-types/media-type such as http://www.iana.org/assignments/media-types/text/calendar. Otherwise, it can be any URL that describes the target format."""@en;
  rdfs:domain csvw:Template;
  rdfs:range xsd:anyURI;
  rdfs:isDefinedBy csvw: .
csvw:templateFormat a rdf:Property;
  rdfs:label "template format"@en;
  rdfs:comment """A URL for the format that is used by the template. If one has been defined, this should be a URL for a media type, in the form http://www.iana.org/assignments/media-types/media-type such as http://www.iana.org/assignments/media-types/application/javascript. Otherwise, it can be any URL that describes the template format."""@en;
  rdfs:domain csvw:Template;
  rdfs:range xsd:anyURI;
  rdfs:isDefinedBy csvw: .
csvw:templates a rdf:Property;
  rdfs:label "templates"@en;
  rdfs:comment """An array of template specifications that provide mechanisms to transform the tabular data into other formats. """@en;
  rdfs:domain [ owl:unionOf (csvw:TableGroup csvw:Table)];
  rdfs:range csvw:Template;
  rdfs:isDefinedBy csvw: .
csvw:text-direction a rdf:Property;
  rdfs:label "text direction"@en;
  rdfs:comment """One of csvw:rtl or csvw:ltr. Indicates whether the text within cells should be displayed by default as left-to-right or right-to-left text. """@en;
  rdfs:domain [ owl:unionOf (csvw:TableGroup csvw:Table csvw:Schema csvw:Column)];
  rdfs:range csvw:Direction;
  rdfs:isDefinedBy csvw: .
csvw:title a rdf:Property;
  rdfs:label "title"@en;
  rdfs:comment """For a Template: A natural language property that describes the format that will be generated from the transformation. This is useful if the target format is a generic format (such as application/json) and the transformation is creating a specific profile of that format.

For a Column: A natural language property that provides possible alternative names for the column."""@en;
  rdfs:domain [ owl:unionOf (csvw:Template csvw:Column)];
  rdfs:isDefinedBy csvw: .
csvw:trim a rdf:Property;
  rdfs:label "trim"@en;
  rdfs:comment """Indicates whether to trim whitespace around cells; may be true, false, start or end. The default is false."""@en;
  rdfs:domain csvw:Dialect;
  rdfs:range xsd:boolean;
  rdfs:isDefinedBy csvw: .
csvw:url a rdf:Property;
  rdfs:label "url"@en;
  rdfs:comment """For a Table: This link property gives the single URL of the CSV file that the table is held in, relative to the location of the metadata document.

For a Template: A link property giving the single URL of the file that the template is held in, relative to the location of the metadata document."""@en;
  rdfs:domain [ owl:unionOf (csvw:Table csvw:Template)];
  rdfs:range xsd:anyURI;
  rdfs:isDefinedBy csvw: .
csvw:valueUrl a rdf:Property;
  rdfs:label "valueUrl"@en;
  rdfs:comment """An URI template property that is used to define one or more resources value of a cell instead of a literal values."""@en;
  rdfs:domain [ owl:unionOf (csvw:TableGroup csvw:Table csvw:Schema csvw:Column)];
  rdfs:range csvw:uriTemplate;
  rdfs:isDefinedBy csvw: .

# Datatype definitions
csvw:json a rdfs:Datatype;
  rdfs:label "json"@en;
  rdfs:comment """A literal containing JSON."""@en;
  rdfs:subClassOf rdfs:Literal;
  rdfs:isDefinedBy csvw: .
csvw:uriTemplate a rdfs:Datatype;
  rdfs:label "uri template"@en;
  rdfs:comment """"""@en;
  rdfs:subClassOf xsd:anyURI;
  rdfs:isDefinedBy csvw: .

# Instance definitions
csvw:ltr a csvw:Direction;
  rdfs:label "left to right"@en;
  rdfs:comment """Indicates text should be processed left to right."""@en;
  rdfs:isDefinedBy csvw: .
csvw:rtl a csvw:Direction;
  rdfs:label "right to left"@en;
  rdfs:comment """Indiects text should be processed right to left"""@en;
  rdfs:isDefinedBy csvw: .
